isabelle_afp/Refine_Monadic/Refine_Heuristics.thy
@@ -152,21 +152,26 @@ lemma prod_rel_iff[refine_hsimp]:
   "((a,b),(a',b'))\<in>\<langle>A,B\<rangle>prod_rel \<longleftrightarrow> (a,a')\<in>A \<and> (b,b')\<in>B"
   by (auto simp: prod_rel_def)
 
+lemmas [refine_hsimp] = prod_rel_id_simp 
+
 lemma option_rel_RELATES[refine_dref_RELATES]: 
   "RELATES Ra \<Longrightarrow> RELATES (\<langle>Ra\<rangle>option_rel)"
   by (simp add: RELATES_def option_rel_def)
 
 declare option_rel_sv[refine_hsimp]
 
-declare option_case_refine[refine del]
-lemma option_case_refine_ext[refine]:
+declare case_option_refine[refine del]
+lemma case_option_refine_ext[refine]:
   assumes "(v,v')\<in>\<langle>Ra\<rangle>option_rel"
   assumes "n \<le> \<Down> Rb n'"
   assumes "\<And>x x'. \<lbrakk> v=Some x; v'=Some x'; (x, x') \<in> Ra \<rbrakk> 
     \<Longrightarrow> f x \<le> \<Down> Rb (f' x')"
-  shows "option_case n f v \<le>\<Down>Rb (option_case n' f' v')"
+  shows "case_option n f v \<le>\<Down>Rb (case_option n' f' v')"
   using assms
   by (auto split: option.split simp: option_rel_def)
+
+lemmas [refine_hsimp] = option_rel_id_simp
+
 
 lemmas [refine_hsimp] = set_rel_sv set_rel_csv
 
